src/Term_Defs.v
@@ -16,109 +16,92 @@ modify it under the terms of the BSD License as published by the
 University of California.  See license.txt for details. *)
 
 Require Import Maps EqClass List ID_Type Defs.
-Import ListNotations.
+Import ListNotations ResultNotation.
 
 Require Export Params_Admits.
 
 Require Export Term_Defs_Core.
 
+Fixpoint appr_asp_to_core (cm : ASP_Compat_MapT) (e : EvidenceT) 
+    : ResultT Core_Term string :=
+  match e with
+  | mt_evt => resultC (aspc NULLC)
+  | nonce_evt n => resultC (aspc (ASPCC check_nonce_params))
+  | asp_evt p ps e' => 
+    let '(asp_paramsC asp_id args targ_plc targ) := ps in
+    match (map_get cm asp_id) with
+    | None => errC "Compatible Appraisal ASP not found in ASP Compat Map"%string
+    | Some appr_id => resultC (aspc (ASPCC (asp_paramsC appr_id args targ_plc targ)))
+    end
+  | split_evt e1 e2 => 
+      e1' <- appr_asp_to_core cm e1 ;;
+      e2' <- appr_asp_to_core cm e2 ;;
+      resultC (bseqc e1' e2')
+  end.
 
 (**  Translating a primitive Copland phrase to its Core_Term equivalent *)
-Definition asp_term_to_core (a:ASP) : Core_Term :=
+Definition asp_term_to_core (cm : ASP_Compat_MapT) (e : EvidenceT) (a:ASP) 
+    : ResultT Core_Term string :=
   match a with
-  | NULL => aspc NULLC
-  | CPY => aspc CPYC
-  | ASPC sp fwd params =>
+  | NULL => resultC (aspc NULLC)
+  | CPY => resultC (aspc CPYC)
+  | ASPC sp params =>
     match sp with
-    | NONE => lseqc (aspc CLEAR) (aspc (ASPCC fwd params))
-    | ALL => (aspc (ASPCC fwd params))
+    | NONE => resultC (lseqc (aspc CLEAR) (aspc (ASPCC params)))
+    | ALL => resultC ((aspc (ASPCC params)))
     end                
-  | SIG => aspc (ASPCC (EXTD 1) sig_params)
-  | HSH => aspc (ASPCC COMP hsh_params)
-  | ENC q => aspc (ASPCC ENCR (enc_params q))
+  | SIG => resultC (aspc (ASPCC sig_params))
+  | APPR => appr_asp_to_core cm e
+  | HSH => resultC (aspc (ASPCC hsh_params))
+  | ENC q => resultC (aspc (ASPCC (enc_params q)))
   end.
 
 (**  Translating a Copland phrase to its Core_Term equivalent *)
-Fixpoint copland_compile (t:Term) : Core_Term :=
+Fixpoint copland_compile (cm : ASP_Compat_MapT) (e : EvidenceT) (t:Term) 
+    : ResultT Core_Term string :=
   match t with
-  | asp a => (asp_term_to_core a)
-  | appr => apprc
-  | att q t' => attc q t'
+  | asp a => (asp_term_to_core cm e a)
+  | att q t' => resultC (attc q t')
 
-  | lseq t1 t2 => lseqc (copland_compile t1) (copland_compile t2)
+  | lseq t1 t2 => 
+      t1' <- copland_compile cm e t1 ;;
+      t2' <- copland_compile cm e t2 ;;
+      resultC (lseqc t1' t2')
 
   | bseq (ALL,ALL) t1 t2 =>
-    bseqc
-      (copland_compile t1) (copland_compile t2)  
+      t1' <- copland_compile cm e t1 ;;
+      t2' <- copland_compile cm e t2 ;;
+      resultC (bseqc t1' t2')
   | bseq (ALL,NONE) t1 t2 =>
-    bseqc
-      (copland_compile t1)
-      (lseqc (aspc CLEAR) (copland_compile t2))
+      t1' <- copland_compile cm e t1 ;;
+      t2' <- copland_compile cm e t2 ;;
+      resultC (bseqc t1' (lseqc (aspc CLEAR) t2'))
   | bseq (NONE,ALL) t1 t2 =>
-    bseqc
-      (lseqc (aspc CLEAR) (copland_compile t1))
-      (copland_compile t2)
+      t1' <- copland_compile cm e t1 ;;
+      t2' <- copland_compile cm e t2 ;;
+      resultC (bseqc (lseqc (aspc CLEAR) t1') t2')
   | bseq (NONE,NONE) t1 t2 =>
-    bseqc
-      (lseqc (aspc CLEAR) (copland_compile t1))
-      (lseqc (aspc CLEAR) (copland_compile t2))
+      t1' <- copland_compile cm e t1 ;;
+      t2' <- copland_compile cm e t2 ;;
+      resultC (bseqc (lseqc (aspc CLEAR) t1') (lseqc (aspc CLEAR) t2'))
           
   | bpar (ALL,ALL) t1 t2 =>
-    bparc O (copland_compile t1) (copland_compile t2)     
+      t1' <- copland_compile cm e t1 ;;
+      t2' <- copland_compile cm e t2 ;;
+      resultC (bparc O t1' t2')
   | bpar (ALL,NONE) t1 t2 =>
-    bparc O
-      (copland_compile t1)
-      (lseqc (aspc CLEAR) (copland_compile t2))
+      t1' <- copland_compile cm e t1 ;;
+      t2' <- copland_compile cm e t2 ;;
+      resultC (bparc O t1' (lseqc (aspc CLEAR) t2'))
   | bpar (NONE,ALL) t1 t2 =>
-    bparc O
-      (lseqc (aspc CLEAR) (copland_compile t1))
-      (copland_compile t2)
+      t1' <- copland_compile cm e t1 ;;
+      t2' <- copland_compile cm e t2 ;;
+      resultC (bparc O (lseqc (aspc CLEAR) t1') t2')
   | bpar (NONE,NONE) t1 t2 =>
-    bparc O
-      (lseqc (aspc CLEAR) (copland_compile t1))
-      (lseqc (aspc CLEAR) (copland_compile t2))
+      t1' <- copland_compile cm e t1 ;;
+      t2' <- copland_compile cm e t2 ;;
+      resultC (bparc O (lseqc (aspc CLEAR) t1') (lseqc (aspc CLEAR) t2'))
   end.
-
-(**  Calculate the size of an EvidenceT type *)
-Fixpoint et_size (e:EvidenceT): nat :=
-  match e with
-  | mt_evt=> O
-  | nonce_evt _ => 1
-  | asp_evt _ fwd _ e' =>
-    match fwd with
-    | COMP => 1
-    | ENCR => 1
-    | (EXTD n) => n + et_size e'
-    | KILL => 0
-    | KEEP => et_size e'
-    end 
-  | appr_evt e' e'' => (et_size e') + (et_size e'')
-  | split_evt e1 e2 => (et_size e1) + (et_size e2)
-  end.
-
-(**  Type-Tagged Raw EvidenceT representation.  Used as the internal EvidenceT
-     type managed by the CVM to track EvidenceT contents and its structure. *)
-Inductive EvC :=
-| evc: RawEv -> EvidenceT -> EvC.
-
-Definition mt_evc: EvC := (evc [] mt_evt).
-
-Definition get_et (e:EvC) : EvidenceT :=
-  match e with
-  | evc ec et => et
-  end.
-
-Definition get_bits (e:EvC): list BS :=
-  match e with
-  | evc ls _ => ls
-  end.
-
-(** A "well-formed" EvC value is where the length of its raw EvidenceT portion
-    has the proper size (calculated over the EvidenceT Type portion). *)
-Inductive wf_ec : EvC -> Prop :=
-| wf_ec_c: forall (ls:RawEv) et,
-    List.length ls = et_size et ->
-    wf_ec (evc ls et).
 
 Definition splitEv_T_l (sp:Split) (e:EvidenceT) : EvidenceT :=
   match sp with
@@ -138,158 +121,97 @@ Definition sp_ev (sp:SP) (e:EvidenceT) : EvidenceT :=
   | NONE => mt_evt
   end.
 
-(** Helper function for EvidenceT type reference semantics *)
-Definition eval_asp t p e :=
-  match t with
-  | NULL => mt_evt
-  | CPY => e 
-  | ASPC sp fwd params =>
-    match fwd with
-    | KEEP => (sp_ev sp e)
-    | KILL => mt_evt
-    | _ => asp_evt p fwd params (sp_ev sp e)
+Fixpoint appr_procedure (aspCM : ASP_Compat_MapT) (p : Plc) (e:EvidenceT) 
+    : ResultT EvidenceT string :=
+  match e with
+  | mt_evt => resultC mt_evt
+  | nonce_evt n => resultC (asp_evt p check_nonce_params (nonce_evt n))
+  | asp_evt asp_top_plc ps e' => 
+    let '(asp_paramsC asp_id args targ_plc targ) := ps in
+    match (map_get aspCM asp_id) with
+    | None => errC "Compatible Appraisal ASP not found in ASP Compat Map"%string
+    | Some appr_id => 
+      resultC (asp_evt p (asp_paramsC appr_id args targ_plc targ) e)
     end
-  | SIG => asp_evt p (EXTD 1) sig_params e
-  | HSH => asp_evt p COMP hsh_params e
-  | ENC q => asp_evt p ENCR (enc_params q) e
+  | split_evt e1 e2 => 
+      e1' <- appr_procedure aspCM p e1 ;;
+      e2' <- appr_procedure aspCM p e2 ;;
+      resultC (split_evt e1' e2')
+  end.
+
+(** Helper function for EvidenceT type reference semantics *)
+Definition eval_asp (G : ASP_Type_Env) (aspCM : ASP_Compat_MapT) (a : ASP) 
+    (p : Plc) (e : EvidenceT) : ResultT EvidenceT string :=
+  match a with
+  | NULL => resultC mt_evt
+  | CPY => resultC e
+  | ASPC sp params =>
+    let '(asp_paramsC asp_id args targ_plc targ) := params in
+    match map_get G asp_id with
+    | None => errC "ASP Type Signature not found in Environment"%string
+    | Some fwd =>
+      match fwd with
+      | KEEP => resultC (sp_ev sp e)
+      | KILL => resultC mt_evt
+      | _ => resultC (asp_evt p params (sp_ev sp e))
+      end
+    end
+  | APPR => appr_procedure aspCM p e
+  | SIG => resultC (asp_evt p sig_params e)
+  | HSH => resultC (asp_evt p hsh_params e)
+  | ENC q => resultC (asp_evt p (enc_params q) e)
   end.
 
 (** EvidenceT Type denotational reference semantics.
     The EvidenceT associated with a term, a place, and some initial EvidenceT. *)
-Import ResultNotation.
-
-Fixpoint appr_procedure (p : Plc) (e:EvidenceT) (aspCM : ASP_Compat_MapT)
-    : ResultT EvidenceT string :=
-  match e with
-  | mt_evt => resultC mt_evt
-  | nonce_evt n => resultC (nonce_evt n)
-  | asp_evt asp_top_plc fwd ps e' => 
-    let '(asp_paramsC asp_id args targ_plc targ) := ps in
-    (* NOTE: Do we need to be able to invert FWD and ARGS? *)
-    match (map_get aspCM asp_id) with
-    | None => errC "ASP not found"%string
-    | Some appr_id => 
-      e'' <- appr_procedure p e' aspCM ;;
-      resultC (asp_evt p fwd (asp_paramsC appr_id args targ_plc targ) e'')
-    end
-  | appr_evt e' e'' => 
-      new_e <- appr_procedure p e' aspCM ;;
-      resultC (appr_evt new_e e)
-  | split_evt e1 e2 => 
-      e1' <- appr_procedure p e1 aspCM ;;
-      e2' <- appr_procedure p e2 aspCM ;;
-      resultC (split_evt e1' e2')
-  end.
 
 Fixpoint asp_comp_map_supports_ev (aspCM : ASP_Compat_MapT) (e : EvidenceT) :=
   match e with
   | mt_evt => True
   | nonce_evt n => True
-  | asp_evt asp_top_plc fwd ps e' => 
+  | asp_evt asp_top_plc ps e' => 
     let '(asp_paramsC asp_id args targ_plc targ) := ps in
-    (* NOTE: Do we need to be able to invert FWD and ARGS? *)
-    map_get aspCM asp_id <> None /\
-    asp_comp_map_supports_ev aspCM e'
-  | appr_evt e' e'' => 
-    asp_comp_map_supports_ev aspCM e' /\ asp_comp_map_supports_ev aspCM e''
-    (* errC "Appr not implemented... not sure how exactly"%string *)
+    map_get aspCM asp_id <> None
   | split_evt e1 e2 => 
       asp_comp_map_supports_ev aspCM e1 /\ asp_comp_map_supports_ev aspCM e2
   end.
 
 Theorem asp_comp_map_supports_ev_iff_appr_procedure: 
-  forall a p aspCM e,
-  asp_comp_map_supports_ev aspCM e ->
-  asp_comp_map_supports_ev aspCM (eval_asp a p e).
+  forall e p aspCM,
+  asp_comp_map_supports_ev aspCM e <->
+  exists e', appr_procedure aspCM p e = resultC e'.
+Proof.
+  induction e; simpl in *; intros; try (intuition; eauto; ffa; fail).
+  - ff; intuition; try congruence; break_exists; try congruence;
+    result_monad_unfold; ff.
+  - ff; intuition; try congruence; break_exists; try congruence;
+    result_monad_unfold; ff;
+    try erewrite IHe1 in *;
+    try erewrite IHe2 in *;
+    break_exists; repeat find_rewrite; try congruence;
+    try (eexists; repeat find_rewrite; eauto; fail).
+    * rewrite Heqr in H; congruence.
+    * rewrite Heqr0 in H0; congruence. 
+  Unshelve. all: eauto.
+Qed.
 
-Fixpoint eval (t:Term) (p:Plc) (e:EvidenceT) (aspCM : ASP_Compat_MapT)
-    : ResultT EvidenceT string :=
+Fixpoint eval (G : ASP_Type_Env) (aspCM : ASP_Compat_MapT) 
+    (t:Term) (p:Plc) (e:EvidenceT) : ResultT EvidenceT string :=
   match t with
-  | asp a => resultC (eval_asp a p e)
-  | att q t1 => eval t1 q e aspCM
-  | appr => 
-      e' <- appr_procedure p e aspCM ;;
-      resultC (appr_evt e' e)
+  | asp a => eval_asp G aspCM a p e
+  | att q t1 => eval G aspCM t1 q e
   | lseq t1 t2 => 
-      e1 <- eval t1 p e aspCM ;;
-      eval t2 p e1 aspCM
+      e1 <- eval G aspCM t1 p e ;;
+      eval G aspCM t2 p e1 
   | bseq s t1 t2 => 
-      e1 <- eval t1 p (splitEv_T_l s e) aspCM ;; 
-      e2 <- eval t2 p (splitEv_T_r s e) aspCM ;;
+      e1 <- eval G aspCM t1 p (splitEv_T_l s e) ;; 
+      e2 <- eval G aspCM t2 p (splitEv_T_r s e) ;;
       resultC (split_evt e1 e2)
   | bpar s t1 t2 => 
-      e1 <- eval t1 p (splitEv_T_l s e) aspCM ;; 
-      e2 <- eval t2 p (splitEv_T_r s e) aspCM ;;
+      e1 <- eval G aspCM t1 p (splitEv_T_l s e) ;; 
+      e2 <- eval G aspCM t2 p (splitEv_T_r s e) ;;
       resultC (split_evt e1 e2)
   end.
-
-
-(* Lemma asp_comp_map_supports_ev_eval_asp : 
-  forall a p aspCM e,
-  asp_comp_map_supports_ev aspCM e ->
-  asp_comp_map_supports_ev aspCM (eval_asp a p e).
-Proof.
-  destruct a; simpl in *; intuition; ff; eauto;
-  unfold sp_ev; ff; intuition.
-
-Lemma asp_comp_map_supports_ev_step : 
-  forall t p aspCM e e',
-  eval t p e aspCM = resultC e' ->
-  asp_comp_map_supports_ev aspCM e ->
-  asp_comp_map_supports_ev aspCM e'.
-Proof.
-  induction t; simpl in *; intuition; eauto; ffa using result_monad_unfold.
-  - 
-  - eapply IHt1 in Heqr; intuition; eauto;
-    unfold splitEv_T_l, splitEv_T_r in *;
-    ff;
-    eapply IHt2 in Heqr0; intuition; eauto; 
-    unfold asp_comp_map_supports_ev; eauto.
-  - eapply IHt1 in Heqr; intuition; eauto;
-    unfold splitEv_T_l, splitEv_T_r in *;
-    ff;
-    eapply IHt2 in Heqr0; intuition; eauto; 
-    unfold asp_comp_map_supports_ev; eauto.
-  - eapply IHt1 in Heqr; intuition; eauto;
-    unfold splitEv_T_l, splitEv_T_r in *;
-    ff;
-    eapply IHt2 in Heqr0; intuition; eauto; 
-    unfold asp_comp_map_supports_ev; eauto.
-  -  
-    eauto.
-    unfold splitEv_T_r in *.
-  induction e; simpl in *; intuition.
-*)
-Lemma eval_res_impl_asp_comp_map_supports_ev : forall t p e aspCM e',
-  asp_comp_map_supports_ev aspCM e ->
-  eval t p e aspCM = resultC e' ->
-  asp_comp_map_supports_ev aspCM e'.
-Proof.
-  induction t; simpl in *; intuition; eauto; ffa using result_monad_unfold.
-  - destruct a; simpl in *; intuition; ff; unfold sp_ev; ff; intuition.
-
-Lemma asp_comp_map_supports_ev_step : 
-  forall t2 t1 aspCM e e' e'' p,
-  asp_comp_map_supports_ev aspCM e ->
-  eval t1 p e aspCM = resultC e' ->
-  eval t2 p e aspCM = resultC e'' ->
-  exists e''', eval t2 p e' aspCM = resultC e'''.
-Proof.
-  intros.
-
-
-Lemma asp_comp_map_supports_term_eval:
-  forall aspCM t p e,
-    asp_comp_map_supports_eval aspCM t e ->
-    exists e', eval t p e aspCM = resultC e'.
-Proof.
-  unfold asp_comp_map_supports_eval.
-  induction t; simpl in *; intuition; eauto; ffa using result_monad_unfold.
-  - admit. 
-  - edestruct IHt1; intuition; eauto; ff.
-    rewrite H0 in Heqr; find_injection.
-    edestruct IHt2; intuition; eauto; ff.
-  unfold appr_procedure in *.
 
 (** * Events
 
@@ -307,7 +229,6 @@ Inductive Ev :=
 | null: nat -> Plc -> Ev
 | copy:  nat -> Plc -> Ev 
 | umeas: nat -> Plc -> ASP_PARAMS -> EvidenceT -> Ev
-| appr_ev : nat -> Plc -> EvidenceT -> Ev
 | req: nat -> Plc -> Plc -> Term -> EvidenceT -> Ev
 | rpy: nat -> Plc -> Plc -> EvidenceT -> Ev 
 | split: nat -> Plc -> Ev
@@ -322,7 +243,6 @@ Definition ev x : nat :=
   | null i _ => i
   | copy i _ => i
   | umeas i _ _ _ => i
-  | appr_ev i _ _ => i
   | req i _ _ _ _ => i
   | rpy i _ _ _ => i 
   | split i _ => i
@@ -353,12 +273,29 @@ See Lemma [events_injective].
  *)
 
 
-Definition asp_event i x p e :=
-  match x with
-  | NULL => null i p
-  | CPY => copy i p
-  | ASPC sp _ ps => umeas i p ps (sp_ev sp e)
-  | SIG => umeas i p sig_params e
-  | HSH => umeas i p hsh_params e
-  | ENC q => umeas i p (enc_params q) e
+Fixpoint asp_event (aspCM : ASP_Compat_MapT) (i : nat) (a : ASP) 
+    (p : Plc) (e : EvidenceT) : ResultT Ev string :=
+  match a with
+  | NULL => resultC (null i p)
+  | CPY => resultC (copy i p)
+  | ASPC sp ps => resultC (umeas i p ps (sp_ev sp e))
+  | APPR => 
+    match e with
+    | mt_evt => resultC (null i p)
+    | nonce_evt n => resultC (umeas i p check_nonce_params (nonce_evt n))
+    | asp_evt p' ps e' => 
+      let '(asp_paramsC asp_id args targ_plc targ) := ps in
+      match (map_get aspCM asp_id) with
+      | None => errC "Compatible Appraisal ASP not found in ASP Compat Map"%string
+      | Some appr_id => 
+        resultC (umeas i p (asp_paramsC appr_id args targ_plc targ) e)
+      end
+    | split_evt e1 e2 => 
+        e1' <- asp_event aspCM i a p e1 ;;
+        e2' <- asp_event aspCM i a p e2 ;;
+        resultC (join i p)
+    end
+  | SIG => resultC (umeas i p sig_params e)
+  | HSH => resultC (umeas i p hsh_params e)
+  | ENC q => resultC (umeas i p (enc_params q) e)
   end.
