src/External_Facts.v
@@ -11,14 +11,14 @@ Import ListNotations.
 
 
 (* TODO: This seems obscenely strong!? *)
-Axiom build_cvm_external' : forall (t : Core_Term) (e : EvC) (tr:list Ev) (i:Event_ID) (ac : Session_Config),
+Axiom build_cvm_external' : forall (t : Core_Term) (e : Evidence) (tr:list Ev) (i:Event_ID) (ac : Session_Config),
   build_cvm t {| st_ev := e; st_trace := tr; st_evid := i; st_config := ac |} 
     = (resultC tt, {| st_ev := cvm_EvidenceT_core t (session_plc ac) e;
            st_trace := tr ++ (cvm_events_core t (session_plc ac) (get_et e));
            st_evid := (i + event_id_span t);
            st_config := ac |}).
 
-Lemma build_cvm_external : forall (t : Core_Term) (e : EvC) i ac,
+Lemma build_cvm_external : forall (t : Core_Term) (e : Evidence) i ac,
     build_cvm t
                     {| st_ev := e;
                        st_trace := [];
